src/lib/poly/gemm/Kuiper.Poly.GEMM.TensorCore.fst
@@ -147,14 +147,11 @@ let barrier_tok
   (l2 : full_mlayout bk bn)
   (sar1 : gpu_array et (bm * bk))
   (sar2 : gpu_array et (bk * bn))
-  (it : nat)
   (nthr : pos)
-  (tid : natlt nthr)
   : slprop
   =
   B.barrier_tok (barrier_p (from_array l1 sar1) (from_array l2 sar2) nthr)
                 (barrier_q (from_array l1 sar1) (from_array l2 sar2) nthr)
-                it tid
 
 unfold
 let kpre
@@ -184,7 +181,8 @@ let kpre
   kpre1 gA eA gB eB gC bm bn bk tm tn tk fA fB bid tid **
   (exists* (x : seq _). gpu_pts_to_array (fst sh)       #(1.0R /. (bm/tm*(bn/tn)*warp_size)) x) **
   (exists* (x : seq _). gpu_pts_to_array (fst (snd sh)) #(1.0R /. (bm/tm*(bn/tn)*warp_size)) x) **
-  barrier_tok (R.row_major bm bk) (R.row_major bk bn) (fst sh) (fst (snd sh)) 0 (bm/tm * (bn/tn) * warp_size) tid
+  barrier_tok (R.row_major bm bk) (R.row_major bk bn) (fst sh) (fst (snd sh)) (bm/tm * (bn/tn) * warp_size) **
+  B.barrier_state 0
 
 unfold
 let kpost
@@ -213,7 +211,8 @@ let kpost
   kpost1 gA eA gB eB gC bm bn tm tn fA fB bid tid **
   exists* (x : seq _). fst sh |-> Frac (1.0R /. (bm/tm*(bn/tn)*warp_size)) x **
   exists* (x : seq _). fst (snd sh) |-> Frac (1.0R /. (bm/tm*(bn/tn)*warp_size)) x **
-  barrier_tok (R.row_major bm bk) (R.row_major bk bn) (fst sh) (fst (snd sh)) (2 * (shared/bk)) (bm/tm*(bn/tn)*warp_size) tid
+  barrier_tok (R.row_major bm bk) (R.row_major bk bn) (fst sh) (fst (snd sh)) (bm/tm * (bn/tn) * warp_size) **
+  B.barrier_state (2 * (shared/bk))
 
 inline_for_extraction noextract
 fn subproducts_tc
@@ -380,7 +379,7 @@ fn kf
   // assert (rewrites_to slA (R.row_major bm bk));
   // let slB = R.row_major bk bn;
   // assert (rewrites_to slB (R.row_major bk bn));
-  unfold barrier_tok (R.row_major bm bk) (R.row_major bk bn) sarA sarB 0 (bm/tm * (bn/tn) * warp_size) tid;
+  unfold barrier_tok (R.row_major bm bk) (R.row_major bk bn) sarA sarB (bm/tm * (bn/tn) * warp_size);
 
   gpu_matrix_abs' (R.row_major bm bk) sarA;
   let sA = from_array (R.row_major bm bk) sarA;
@@ -423,10 +422,8 @@ fn kf
         accumFrag |-> vaccumFrag **
         (exists* (x : ematrix _ _ _). sA |-> Frac (1.0R /. ((bm/tm*(bn/tn) * warp_size))) x) **
         (exists* (x : ematrix _ _ _). sB |-> Frac (1.0R /. ((bm/tm*(bn/tn) * warp_size))) x) **
-        B.barrier_tok (barrier_p sA sB ((bm/tm*(bn/tn)* warp_size))) (barrier_q sA sB ((bm/tm*(bn/tn) * warp_size))) (2 * !bkIdx) tid
+        B.barrier_state (2 * !bkIdx)
   {
-    (* This assert should not be needed. I don't know what effect it even has. *)
-    assert B.barrier_tok (barrier_p sA sB (bm/tm * (bn/tn) * warp_size)) (barrier_q sA sB (bm/tm * (bn/tn) * warp_size)) (2 * !bkIdx) tid;
     even_2x !bkIdx;
     assert pure((2 * !bkIdx % 2 = 0) == true);
     rewrite
@@ -441,7 +438,7 @@ fn kf
 
     copy_tiles_out_of_matrices bm bn bk sA sB gA gB mrow !bkIdx mcol (bm/^tm*^(bn/^tn)*^warp_sz) tid;
 
-    assert (B.barrier_tok (barrier_p sA sB (bm/tm * (bn/tn) * warp_size)) (barrier_q sA sB (bm/tm * (bn/tn) * warp_size)) (2 * !bkIdx + 1) tid);
+    assert (B.barrier_tok (barrier_p sA sB (bm/tm * (bn/tn) * warp_size)) (barrier_q sA sB (bm/tm * (bn/tn) * warp_size)));
     odd_2x1 !bkIdx;
     assert (pure (odd (2 * !bkIdx + 1)));
     rewrite live_strided_chunks sA (bm/tm * (bn/tn) * warp_size) tid **
@@ -477,18 +474,14 @@ fn kf
   rewrite
     B.barrier_tok (barrier_p sA sB (v bm / v tm * (v bn / v tn) * 32))
       (barrier_q sA sB (v bm / v tm * (v bn / v tn) * 32))
-      (2 * v !bkIdx)
-      (v tid)
   as
     B.barrier_tok (barrier_p (from_array (R.row_major (v bm) (v bk)) sarA)
           (from_array (R.row_major (v bk) (v bn)) sarB)
           (v bm / v tm * (v bn / v tn) * 32))
       (barrier_q (from_array (R.row_major (v bm) (v bk)) sarA)
           (from_array (R.row_major (v bk) (v bn)) sarB)
-          (v bm / v tm * (v bn / v tn) * 32))
-      (2 * (shared / bk))
-      (v tid);
-  fold barrier_tok (R.row_major bm bk) (R.row_major bk bn) sarA sarB (2 * (shared / bk)) (bm/tm * (bn/tn) * warp_size) tid;
+          (v bm / v tm * (v bn / v tn) * 32));
+  fold barrier_tok (R.row_major bm bk) (R.row_major bk bn) sarA sarB (bm/tm * (bn/tn) * warp_size);
 
   rewrite each sarA as fst sh;
   rewrite each sarB as fst (snd sh);
